libcrux-ml-kem/proofs/fstar/extraction/Libcrux_ml_kem.Vector.Avx2.fsti
@@ -10,7 +10,6 @@ let _ =
   ()
 
 noeq
-
 type t_SIMD256Vector = { f_elements:Libcrux_intrinsics.Avx2_extract.t_Vec256 }
 
 let repr (x:t_SIMD256Vector) : t_Array i16 (sz 16) = Libcrux_intrinsics.Avx2_extract.vec256_as_i16x16 x.f_elements
@@ -173,6 +172,7 @@ let impl_3: Libcrux_ml_kem.Vector.Traits.t_Operations t_SIMD256Vector =
     f_cond_subtract_3329_
     =
     (fun (vector: t_SIMD256Vector) ->
+        let _:Prims.unit = admit () in
         { f_elements = Libcrux_ml_kem.Vector.Avx2.Arithmetic.cond_subtract_3329_ vector.f_elements }
         <:
         t_SIMD256Vector);
@@ -273,6 +273,7 @@ let impl_3: Libcrux_ml_kem.Vector.Traits.t_Operations t_SIMD256Vector =
     f_ntt_layer_1_step
     =
     (fun (vector: t_SIMD256Vector) (zeta0: i16) (zeta1: i16) (zeta2: i16) (zeta3: i16) ->
+        let _:Prims.unit = admit () in
         {
           f_elements
           =
@@ -292,6 +293,7 @@ let impl_3: Libcrux_ml_kem.Vector.Traits.t_Operations t_SIMD256Vector =
     f_ntt_layer_2_step
     =
     (fun (vector: t_SIMD256Vector) (zeta0: i16) (zeta1: i16) ->
+        let _:Prims.unit = admit () in
         {
           f_elements = Libcrux_ml_kem.Vector.Avx2.Ntt.ntt_layer_2_step vector.f_elements zeta0 zeta1
         }
@@ -309,6 +311,7 @@ let impl_3: Libcrux_ml_kem.Vector.Traits.t_Operations t_SIMD256Vector =
     f_ntt_layer_3_step
     =
     (fun (vector: t_SIMD256Vector) (zeta: i16) ->
+        let _:Prims.unit = admit () in
         { f_elements = Libcrux_ml_kem.Vector.Avx2.Ntt.ntt_layer_3_step vector.f_elements zeta }
         <:
         t_SIMD256Vector);
@@ -332,6 +335,7 @@ let impl_3: Libcrux_ml_kem.Vector.Traits.t_Operations t_SIMD256Vector =
     f_inv_ntt_layer_1_step
     =
     (fun (vector: t_SIMD256Vector) (zeta0: i16) (zeta1: i16) (zeta2: i16) (zeta3: i16) ->
+        let _:Prims.unit = admit () in
         {
           f_elements
           =
@@ -355,6 +359,7 @@ let impl_3: Libcrux_ml_kem.Vector.Traits.t_Operations t_SIMD256Vector =
     f_inv_ntt_layer_2_step
     =
     (fun (vector: t_SIMD256Vector) (zeta0: i16) (zeta1: i16) ->
+        let _:Prims.unit = admit () in
         {
           f_elements
           =
@@ -373,6 +378,7 @@ let impl_3: Libcrux_ml_kem.Vector.Traits.t_Operations t_SIMD256Vector =
     f_inv_ntt_layer_3_step
     =
     (fun (vector: t_SIMD256Vector) (zeta: i16) ->
+        let _:Prims.unit = admit () in
         { f_elements = Libcrux_ml_kem.Vector.Avx2.Ntt.inv_ntt_layer_3_step vector.f_elements zeta }
         <:
         t_SIMD256Vector);
@@ -412,6 +418,7 @@ let impl_3: Libcrux_ml_kem.Vector.Traits.t_Operations t_SIMD256Vector =
         (zeta2: i16)
         (zeta3: i16)
         ->
+        let _:Prims.unit = admit () in
         {
           f_elements
           =
@@ -435,7 +442,7 @@ let impl_3: Libcrux_ml_kem.Vector.Traits.t_Operations t_SIMD256Vector =
     f_serialize_1_
     =
     (fun (vector: t_SIMD256Vector) ->
-        let _:Prims.unit = admit () in
+       admit ();
         Libcrux_ml_kem.Vector.Avx2.Serialize.serialize_1_ vector.f_elements);
     f_deserialize_1_pre
     =
@@ -447,7 +454,7 @@ let impl_3: Libcrux_ml_kem.Vector.Traits.t_Operations t_SIMD256Vector =
     f_deserialize_1_
     =
     (fun (bytes: t_Slice u8) ->
-        let _:Prims.unit = admit () in
+       admit ();
         { f_elements = Libcrux_ml_kem.Vector.Avx2.Serialize.deserialize_1_ bytes }
         <:
         t_SIMD256Vector);
@@ -462,7 +469,6 @@ let impl_3: Libcrux_ml_kem.Vector.Traits.t_Operations t_SIMD256Vector =
     f_serialize_4_
     =
     (fun (vector: t_SIMD256Vector) ->
-        let _:Prims.unit = admit () in
         Libcrux_ml_kem.Vector.Avx2.Serialize.serialize_4_ vector.f_elements);
     f_deserialize_4_pre
     =
@@ -474,7 +480,6 @@ let impl_3: Libcrux_ml_kem.Vector.Traits.t_Operations t_SIMD256Vector =
     f_deserialize_4_
     =
     (fun (bytes: t_Slice u8) ->
-        let _:Prims.unit = admit () in
         { f_elements = Libcrux_ml_kem.Vector.Avx2.Serialize.deserialize_4_ bytes }
         <:
         t_SIMD256Vector);
@@ -483,6 +488,7 @@ let impl_3: Libcrux_ml_kem.Vector.Traits.t_Operations t_SIMD256Vector =
     f_serialize_5_
     =
     (fun (vector: t_SIMD256Vector) ->
+        let _:Prims.unit = admit () in
         Libcrux_ml_kem.Vector.Avx2.Serialize.serialize_5_ vector.f_elements);
     f_deserialize_5_pre
     =
@@ -491,6 +497,7 @@ let impl_3: Libcrux_ml_kem.Vector.Traits.t_Operations t_SIMD256Vector =
     f_deserialize_5_
     =
     (fun (bytes: t_Slice u8) ->
+        let _:Prims.unit = admit () in
         { f_elements = Libcrux_ml_kem.Vector.Avx2.Serialize.deserialize_5_ bytes }
         <:
         t_SIMD256Vector);
@@ -505,7 +512,6 @@ let impl_3: Libcrux_ml_kem.Vector.Traits.t_Operations t_SIMD256Vector =
     f_serialize_10_
     =
     (fun (vector: t_SIMD256Vector) ->
-        let _:Prims.unit = admit () in
         Libcrux_ml_kem.Vector.Avx2.Serialize.serialize_10_ vector.f_elements);
     f_deserialize_10_pre
     =
@@ -517,7 +523,6 @@ let impl_3: Libcrux_ml_kem.Vector.Traits.t_Operations t_SIMD256Vector =
     f_deserialize_10_
     =
     (fun (bytes: t_Slice u8) ->
-        let _:Prims.unit = admit () in
         { f_elements = Libcrux_ml_kem.Vector.Avx2.Serialize.deserialize_10_ bytes }
         <:
         t_SIMD256Vector);
@@ -548,7 +553,6 @@ let impl_3: Libcrux_ml_kem.Vector.Traits.t_Operations t_SIMD256Vector =
     f_serialize_12_
     =
     (fun (vector: t_SIMD256Vector) ->
-        let _:Prims.unit = admit () in
         Libcrux_ml_kem.Vector.Avx2.Serialize.serialize_12_ vector.f_elements);
     f_deserialize_12_pre
     =
@@ -560,7 +564,6 @@ let impl_3: Libcrux_ml_kem.Vector.Traits.t_Operations t_SIMD256Vector =
     f_deserialize_12_
     =
     (fun (bytes: t_Slice u8) ->
-        let _:Prims.unit = admit () in
         { f_elements = Libcrux_ml_kem.Vector.Avx2.Serialize.deserialize_12_ bytes }
         <:
         t_SIMD256Vector);
